src/LamRefLogicFactsTotal.v
@@ -10,7 +10,7 @@ Require Import src.LambdaTotalTriple.
 
 (*
 (*total correctness*)
-Theorem triple_weaken (V : Set) (e : Expr V) P P' Q Q' :
+Theorem htriple_weaken (V : Set) (e : Expr V) P P' Q Q' :
   sa_implies P' P ->
   (forall v c, sa_implies (Q v c) (Q' v c)) ->
   hoare_triple e P Q ->
@@ -20,21 +20,21 @@ Proof.
   edestruct Hhoare as [? [? ?]]; eauto.
 Qed.
 
-Theorem triple_value (V : Set) (v : Value V) (P : StateAssertion V) :
+Theorem htriple_value (V : Set) (v : Value V) (P : StateAssertion V) :
   hoare_triple v P (fun _ c => sa_star (sa_pure (c = 0)) P).
 Proof.
   unfold hoare_triple, sa_star, sa_pure, sa_empty, disjoint_maps.
   intros v' m p. repeat eexists; eauto.
 Qed.
 
-Theorem triple_value' (V : Set) (v : Value V) :
+Theorem htriple_value' (V : Set) (v : Value V) :
   hoare_triple v sa_empty (fun _ c => sa_pure (c = 0)).
 Proof.
   unfold hoare_triple, sa_pure, sa_empty.
   intros v' m p. repeat eexists.
 Qed.
 *)
-
+(*
 Ltac inversion_red :=
   match goal with
   | [H : red _ _ _ _ |- _] =>
@@ -54,64 +54,11 @@ Ltac find_red_cases :=
 
 Ltac solve_red_cases :=
   find_red_cases; inversion_cost_red; subst; auto; discriminate_red_Val.
-
-
-Theorem triple_weaken (V : Set) (e : Expr V) P P' Q Q' :
-  P' ->> P ->
-  (forall v c, (Q v c) ->> (Q' v c)) ->
-  hoare_triple e P Q ->
-  hoare_triple e P' Q'.
-Proof.
-  unfold hoare_triple, sa_implies. intros ? ? H ? ?.
-  edestruct H as [? [? [? [? ?]]]]; eauto 10.
-Qed.
-
-Theorem triple_value (V : Set) (v : Value V) :
-  hoare_triple v <[]> (fun v' c => <[v' = v /\ c = 0]>).
-Proof.
-  unfold hoare_triple, sa_pure, sa_empty.
-  intros m Hm. subst. eauto 10 with lamref.
-Qed.
-
-Theorem triple_value' (V : Set) (v : Value V) (P : StateAssertion V) :
-  hoare_triple v P (fun v' c => <[v' = v /\ c = 0]> <*> P).
-Proof.
-  unfold hoare_triple, sa_star, sa_pure, sa_empty, disjoint_maps.
-  eauto 15 with lamref.
-Qed.
-
-Theorem triple_value_untimed (V : Set) (v : Value V) (P : StateAssertion V) :
-  hoare_triple v P (fun _ _ => P).
-Proof.
-  eapply triple_weaken; eauto using triple_value';
-    unfold sa_implies, sa_star, sa_pure, sa_empty;
-    [| intros v' c m [m1 [m2 [[? ?] [? [? ?]]]]]; subst ];
-    eauto.
-Qed.
-
-Theorem triple_lam (V : Set) (e : Expr _) (v : Value V) P Q :
-  hoare_triple (subst_e e v) P (fun v c => Q v (1+c)) ->
-  hoare_triple ((-\e) <* v) P Q.
-Proof.
-  unfold hoare_triple. intros.
-  edestruct H as [? [? [? [? ?]]]]; eauto 10 with lamref.
-Qed.
-
-(*Theorem triple_seq (V : Set) (e1 e2 : Expr V) P1 P2 Q1 Q2 :
-  hoare_triple e1 P1 Q1 ->
-  hoare_triple e2 P2 Q2 ->
-  (forall v c, Q1 v c ->> P1) ->
-  hoare_triple (e1 ;; e2) P1 Q2.
-Proof.
-  unfold hoare_triple, sa_exists, sa_star, sa_single, sa_pure, sa_empty,
-    disjoint_maps.
-  intros.
-  inversion_cost_red. inversion_red.
 *)
 
 Ltac unfold_all :=
-  unfold hoare_triple, sa_exists, sa_star, sa_single, sa_pure, sa_empty,
-    sa_implies, disjoint_maps, labels.
+  unfold triple, hoare_triple, sa_exists, sa_star, sa_single, sa_pure,
+    sa_empty, sa_implies, disjoint_maps, labels.
 
 Ltac edestruct_direct :=
   repeat match goal with
@@ -137,7 +84,180 @@ Ltac solve_triple n H :=
 
 Ltac solve_triple_15 := solve_triple integer:(15).
 
-Theorem triple_app (V : Set) (e1 e2 : Expr V) e1' (v2 : Value V)
+Theorem htriple_of_triple (V : Set) (e : Expr V) P Q :
+  triple e P Q ->
+  hoare_triple e P Q.
+Proof.
+  unfold triple. intros Htriple. specialize Htriple with <[]>. revert Htriple.
+  unfold_all. intros. edestruct_all_in integer:(10).
+  repeat rewrite List.app_nil_r in *. eauto.
+Qed.
+
+Theorem htriple_weaken (V : Set) (e : Expr V) P P' Q Q' :
+  P' ->> P ->
+  (forall v c, (Q v c) ->> (Q' v c)) ->
+  hoare_triple e P Q ->
+  hoare_triple e P' Q'.
+Proof.
+  unfold hoare_triple, sa_implies. intros ? ? H ? ?.
+  edestruct H as [? [? [? [? ?]]]]; eauto 10.
+Qed.
+
+Lemma implies_refl V (P : StateAssertion V) : P ->> P.
+Proof.
+  now unfold_all.
+Qed.
+
+Lemma star_implies_mono V (P : StateAssertion V) P' Q Q' :
+  P ->> P' ->
+  Q ->> Q' ->
+  P <*> Q ->> P' <*> Q'.
+Proof.
+  unfold_all. intros. edestruct_direct. eauto 10.
+Qed.
+
+Lemma star_implies_mono_post
+  (V : Set) (P : V -> nat -> StateAssertion V) P' Q Q' :
+  P -->> P' ->
+  Q ->> Q' ->
+  P <*>+ Q -->> P' <*>+ Q'.
+Proof.
+  intros. now apply star_implies_mono.
+Qed.
+
+Theorem triple_weaken (V : Set) (e : Expr V) P P' Q Q' :
+  P' ->> P ->
+  (forall v c, (Q v c) ->> (Q' v c)) ->
+  triple e P Q ->
+  triple e P' Q'.
+Proof.
+  unfold triple. intros.
+  eapply htriple_weaken with (P <*> _) (Q <*>+ _);
+    eauto using star_implies_mono, implies_refl.
+Qed.
+
+Theorem htriple_pure (V : Set) (e : Expr V) P Q :
+  (P -> hoare_triple e <[]> Q) <-> hoare_triple e <[P]> Q.
+Proof.
+  unfold hoare_triple, sa_pure, sa_empty.
+  split; intros ? ? H; [destruct H|]; subst; auto.
+Qed.
+
+Theorem htriple_exists A (V : Set) (e : Expr V) P Q :
+  (forall x : A, hoare_triple e (P x) Q) <->
+    hoare_triple e (<exists> x, P x) Q.
+Proof.
+  unfold hoare_triple, sa_exists. split; intros ? ? H; [destruct H|]; eauto.
+Qed.
+
+Theorem htriple_pure_post (V : Set) (e : Expr V) P Q :
+  ((forall m, P m -> Q) /\ hoare_triple e P (fun _ _ => <[]>)) <->
+    hoare_triple e P (fun _ _ => <[Q]>).
+Proof.
+  unfold hoare_triple, sa_pure, sa_empty. split.
+  - intros [? Hhoare] ? ?.
+    edestruct Hhoare as (?&?&?&?&->); repeat eexists; eauto.
+  - intros Hhoare. split; intros; edestruct Hhoare as (?&?&?&?&?&->); eauto.
+Qed.
+
+Ltac solve_assoc :=
+  repeat eexists; eauto using List.app_assoc; rewrite List.map_app in *; intros;
+    try match goal with
+    | [H : List.In _ (_ ++ _)%list |- _] => apply List.in_app_or in H as [? | ?]
+    end;
+    eauto using List.in_or_app.
+
+Lemma star_assoc_l (V : Set) (P : StateAssertion V) Q R :
+  P <*> (Q <*> R) ->> (P <*> Q) <*> R.
+Proof.
+  unfold_all. intros. edestruct_direct.
+  solve_assoc.
+Qed.
+
+Lemma star_assoc_r (V : Set) (P : StateAssertion V) Q R :
+  (P <*> Q) <*> R ->> P <*> (Q <*> R).
+Proof.
+  unfold_all. intros. edestruct_direct.
+  solve_assoc.
+Qed.
+
+Lemma star_assoc (V : Set) (P : StateAssertion V) Q R :
+  P <*> (Q <*> R) <<->> (P <*> Q) <*> R.
+Proof.
+  auto using star_assoc_l, star_assoc_r.
+Qed.
+
+Lemma star_assoc_post_l (V : Set) (P : V -> nat -> StateAssertion V) Q R :
+  P <*>+ (Q <*> R) -->> (P <*>+ Q) <*>+ R.
+Proof.
+  simpl. auto using star_assoc_l.
+Qed.
+
+Lemma star_assoc_post_r (V : Set) (P : V -> nat -> StateAssertion V) Q R :
+  (P <*>+ Q) <*>+ R -->> P <*>+ (Q <*> R).
+Proof.
+  simpl. auto using star_assoc_r.
+Qed.
+
+Lemma star_assoc_post (V : Set) (P : V -> nat -> StateAssertion V) Q R :
+  P <*>+ (Q <*> R) <<-->> (P <*>+ Q) <*>+ R.
+Proof.
+  auto using star_assoc_post_l, star_assoc_post_r.
+Qed.
+
+Theorem triple_frame (V : Set) (e : Expr V) P Q H :
+  triple e P Q ->
+  triple e (P <*> H) (Q <*>+ H).
+Proof.
+  unfold triple. intros.
+  eapply htriple_weaken with (P <*> (_ <*> _)) (Q <*>+ (_ <*> _));
+    auto using star_assoc_r, star_assoc_l.
+Qed.
+
+Theorem htriple_value (V : Set) (v : Value V) :
+  hoare_triple v <[]> (fun v' c => <[v' = v /\ c = 0]>).
+Proof.
+  unfold hoare_triple, sa_pure, sa_empty.
+  intros m Hm. subst. eauto 10 with lamref.
+Qed.
+
+Theorem htriple_value' (V : Set) (v : Value V) (P : StateAssertion V) :
+  hoare_triple v P (fun v' c => <[v' = v /\ c = 0]> <*> P).
+Proof.
+  unfold hoare_triple, sa_star, sa_pure, sa_empty, disjoint_maps.
+  eauto 15 with lamref.
+Qed.
+
+Theorem htriple_value_untimed (V : Set) (v : Value V) (P : StateAssertion V) :
+  hoare_triple v P (fun _ _ => P).
+Proof.
+  eapply htriple_weaken; eauto using htriple_value';
+    unfold sa_implies, sa_star, sa_pure, sa_empty;
+    [| intros v' c m [m1 [m2 [[? ?] [? [? ?]]]]]; subst ];
+    eauto.
+Qed.
+
+Theorem htriple_lam (V : Set) (e : Expr _) (v : Value V) P Q :
+  hoare_triple (subst_e e v) P (fun v c => Q v (1+c)) ->
+  hoare_triple ((-\e) <* v) P Q.
+Proof.
+  unfold hoare_triple. intros.
+  edestruct H as [? [? [? [? ?]]]]; eauto 10 with lamref.
+Qed.
+
+(*Theorem htriple_seq (V : Set) (e1 e2 : Expr V) P1 P2 Q1 Q2 :
+  hoare_triple e1 P1 Q1 ->
+  hoare_triple e2 P2 Q2 ->
+  (forall v c, Q1 v c ->> P1) ->
+  hoare_triple (e1 ;; e2) P1 Q2.
+Proof.
+  unfold hoare_triple, sa_exists, sa_star, sa_single, sa_pure, sa_empty,
+    disjoint_maps.
+  intros.
+  inversion_cost_red. inversion_red.
+*)
+
+Theorem htriple_app (V : Set) (e1 e2 : Expr V) e1' (v2 : Value V)
   P1 P2 P3 Q3 c1 c2 :
   hoare_triple e1 P1 (fun v c => <[v = (-\e1') /\ c = c1]> <*> P2) ->
   hoare_triple e2 P2 (fun v c => <[v = v2 /\ c = c2]> <*> P3) ->
@@ -147,7 +267,7 @@ Proof.
   solve_triple integer:(10) big_red_app.
 Qed.
 
-Theorem triple_bneg (V : Set) (e : Expr V) (b : bool) P Q :
+Theorem htriple_bneg (V : Set) (e : Expr V) (b : bool) P Q :
   hoare_triple e P (fun v c => <[v = Bool b]> <*> Q (1+c)) ->
   hoare_triple ([~] e)
     P
@@ -156,7 +276,7 @@ Proof.
   solve_triple_15 big_red_bneg.
 Qed.
 
-Theorem triple_ineg (V : Set) (e : Expr V) (i : Z) P Q :
+Theorem htriple_ineg (V : Set) (e : Expr V) (i : Z) P Q :
   hoare_triple e P (fun v c => <[v = Int i]> <*> Q (1+c)) ->
   hoare_triple ([--] e)
     P
@@ -165,7 +285,7 @@ Proof.
   solve_triple_15 big_red_ineg.
 Qed.
 
-Theorem triple_bor (V : Set) (e1 e2 : Expr V) (b1 b2 : bool)
+Theorem htriple_bor (V : Set) (e1 e2 : Expr V) (b1 b2 : bool)
   P1 P2 Q2 c1 :
   hoare_triple e1 P1 (fun v c => <[v = Bool b1 /\ c = c1]> <*> P2) ->
   hoare_triple e2 P2 (fun v c => <[v = Bool b2]> <*> Q2 (c1+c+1)) ->
@@ -176,7 +296,7 @@ Proof.
   solve_triple_15 big_red_bor.
 Qed.
 
-Theorem triple_band (V : Set) (e1 e2 : Expr V) (b1 b2 : bool)
+Theorem htriple_band (V : Set) (e1 e2 : Expr V) (b1 b2 : bool)
   P1 P2 Q2 c1 :
   hoare_triple e1 P1 (fun v c => <[v = Bool b1 /\ c = c1]> <*> P2) ->
   hoare_triple e2 P2 (fun v c => <[v = Bool b2]> <*> Q2 (c1+c+1)) ->
@@ -187,7 +307,7 @@ Proof.
   solve_triple_15 big_red_band.
 Qed.
 
-Theorem triple_iadd (V : Set) (e1 e2 : Expr V) (i1 i2 : Z)
+Theorem htriple_iadd (V : Set) (e1 e2 : Expr V) (i1 i2 : Z)
   P1 P2 Q2 c1 :
   hoare_triple e1 P1 (fun v c => <[v = Int i1 /\ c = c1]> <*> P2) ->
   hoare_triple e2 P2 (fun v c => <[v = Int i2]> <*> Q2 (c1+c+1)) ->
@@ -198,7 +318,7 @@ Proof.
   solve_triple_15 big_red_iadd.
 Qed.
 
-Theorem triple_isub (V : Set) (e1 e2 : Expr V) (i1 i2 : Z)
+Theorem htriple_isub (V : Set) (e1 e2 : Expr V) (i1 i2 : Z)
   P1 P2 Q2 c1 :
   hoare_triple e1 P1 (fun v c => <[v = Int i1 /\ c = c1]> <*> P2) ->
   hoare_triple e2 P2 (fun v c => <[v = Int i2]> <*> Q2 (c1+c+1)) ->
@@ -209,7 +329,7 @@ Proof.
   solve_triple_15 big_red_isub.
 Qed.
 
-Theorem triple_imul (V : Set) (e1 e2 : Expr V) (i1 i2 : Z)
+Theorem htriple_imul (V : Set) (e1 e2 : Expr V) (i1 i2 : Z)
   P1 P2 Q2 c1 :
   hoare_triple e1 P1 (fun v c => <[v = Int i1 /\ c = c1]> <*> P2) ->
   hoare_triple e2 P2 (fun v c => <[v = Int i2]> <*> Q2 (c1+c+1)) ->
@@ -220,7 +340,7 @@ Proof.
   solve_triple_15 big_red_imul.
 Qed.
 
-Theorem triple_idiv (V : Set) (e1 e2 : Expr V) (i1 i2 : Z)
+Theorem htriple_idiv (V : Set) (e1 e2 : Expr V) (i1 i2 : Z)
   P1 P2 Q2 c1 :
   hoare_triple e1 P1 (fun v c => <[v = Int i1 /\ c = c1]> <*> P2) ->
   hoare_triple e2 P2 (fun v c => <[v = Int i2]> <*> Q2 (c1+c+1)) ->
@@ -231,7 +351,7 @@ Proof.
   solve_triple_15 big_red_idiv.
 Qed.
 
-Theorem triple_clt (V : Set) (e1 e2 : Expr V) (i1 i2 : Z)
+Theorem htriple_clt (V : Set) (e1 e2 : Expr V) (i1 i2 : Z)
   P1 P2 Q2 c1 :
   hoare_triple e1 P1 (fun v c => <[v = Int i1 /\ c = c1]> <*> P2) ->
   hoare_triple e2 P2 (fun v c => <[v = Int i2]> <*> Q2 (c1+c+1)) ->
@@ -242,7 +362,7 @@ Proof.
   solve_triple_15 big_red_clt.
 Qed.
 
-Theorem triple_ceq (V : Set) (e1 e2 : Expr V) (i1 i2 : Z)
+Theorem htriple_ceq (V : Set) (e1 e2 : Expr V) (i1 i2 : Z)
   P1 P2 Q2 c1 :
   hoare_triple e1 P1 (fun v c => <[v = Int i1 /\ c = c1]> <*> P2) ->
   hoare_triple e2 P2 (fun v c => <[v = Int i2]> <*> Q2 (c1+c+1)) ->
@@ -277,7 +397,7 @@ Ltac inversion_Nth_cons :=
 
 Ltac inversion_all_Nth_cons := repeat inversion_Nth_cons.
 
-Theorem triple_rec (V : Set) (es : list (Expr V)) (vs : list (Value V))
+Theorem htriple_rec (V : Set) (es : list (Expr V)) (vs : list (Value V))
   n cs Ps P Q :
   n = List.length es ->
   n = List.length vs ->
@@ -332,7 +452,7 @@ Proof.
   eauto 15 using big_red_rec with lamref.
 Qed.
 
-Theorem triple_get (V : Set) n (e : Expr V) (vs : list (Value V)) v P Q :
+Theorem htriple_get (V : Set) n (e : Expr V) (vs : list (Value V)) v P Q :
   Nth n vs v ->
   hoare_triple e P (fun v' c => <[v' = RecV vs]> <*> Q (1+c)) ->
   hoare_triple (Get n e)
@@ -342,7 +462,7 @@ Proof.
   solve_triple_15 big_red_get.
 Qed.
 
-Theorem triple_ref (V : Set) (e : Expr V) (v : Value V) P Q :
+Theorem htriple_ref (V : Set) (e : Expr V) (v : Value V) P Q :
   hoare_triple e P (fun v' c => <[v' = v]> <*> Q (1+c)) ->
   hoare_triple (Ref e)
     P
@@ -354,7 +474,7 @@ Proof.
   intros ? [? | []] ?. subst. eauto.
 Qed.
 
-Theorem triple_deref (V : Set) (e : Expr V) (v : Value V) l P Q :
+Theorem htriple_deref (V : Set) (e : Expr V) (v : Value V) l P Q :
   hoare_triple e
     (<(l :== v)> <*> P)
     (fun v' c => <[v' = Lab l]> <*> <(l :== v)> <*> Q (1+c)) ->
@@ -366,7 +486,7 @@ Proof.
   repeat eexists; try eapply big_red_deref; simpl in *; eauto with lamref.
 Qed.
 
-Theorem triple_assign (V : Set) (e1 e2 : Expr V) (v v' : Value V) l P1 P2 Q2 c1 :
+Theorem htriple_assign (V : Set) (e1 e2 : Expr V) (v v' : Value V) l P1 P2 Q2 c1 :
   hoare_triple e1
     (<(l :== v)> <*> P1)
     (fun v'' c => <[v'' = Lab l /\ c = c1]> <*> <(l :== v)> <*> P2) ->
@@ -384,7 +504,7 @@ Proof.
   auto with lamref.
 Qed.
 
-Theorem triple_seq (V : Set) (e1 e2 : Expr V) (v : Value V) P1 P2 Q2 c1 :
+Theorem htriple_seq (V : Set) (e1 e2 : Expr V) (v : Value V) P1 P2 Q2 c1 :
   hoare_triple e1
     P1
     (fun v' c => <[v' = U_val /\ c = c1]> <*> P2) ->
@@ -398,7 +518,7 @@ Proof.
   solve_triple_15 big_red_seq.
 Qed.
 
-Theorem triple_if (V : Set) (e1 e2 e3 : Expr V) b P1 P2 Q2 c1 :
+Theorem htriple_if_simple (V : Set) (e1 e2 e3 : Expr V) b P1 P2 Q2 c1 :
   hoare_triple e1
     P1
     (fun v' c => <[v' = Bool b /\ c = c1]> <*> P2 b) ->
@@ -415,22 +535,42 @@ Proof.
   - solve_triple_15 big_red_if_false.
 Qed.
 
-(*
-Theorem triple_while_true (V : Set) (e1 e2 : Expr V) P Q :
+Theorem htriple_if (V : Set) (e1 e2 e3 : Expr V) P1 P2 Q2 c1 :
+  hoare_triple e1
+    P1
+    (fun v' c => <exists> b, <[v' = Bool b /\ c = c1]> <*> P2 b) ->
+  hoare_triple e2
+    (P2 true)
+    (fun v c => Q2 v (c1+1+c)) ->
+  hoare_triple e3
+    (P2 false)
+    (fun v c => Q2 v (c1+1+c)) ->
+  hoare_triple (If e1 e2 e3) P1 Q2.
+Proof.
+  unfold_all. intros. edestruct_all.
+  match goal with [b : bool |- _] => destruct b end.
+  - solve_triple_15 big_red_if_true.
+  - solve_triple_15 big_red_if_false.
+Qed.
+
+Theorem htriple_while_true (V : Set) (e1 e2 : Expr V) c1 c2 P P2 P3 Q :
   hoare_triple e1
     P
-    (fun v c => <[v = Bool true]> <*> Q (1+(c+1))) ->
-  hoare_triple e
-    P
-    (fun v c => <[v = Bool true]> <*> Q (1+(c+1))) ->
+    (fun v c => <[v = Bool true /\ c = c1]> <*> P2) ->
+  hoare_triple e2
+    P2
+    (fun v c => <[v = U_val /\ c = c2]> <*> P3) ->
+  hoare_triple (While e1 e2)
+    P3
+    (fun v c => <[v = U_val]> <*> Q (1+(c1+1+(c2+1+c)))) ->
   hoare_triple (While e1 e2)
     P
     (fun v c => <[v = U_val]> <*> Q c).
 Proof.
   solve_triple_15 big_red_while_true.
 Qed.
-*)
-Theorem triple_while_false (V : Set) (e1 e2 : Expr V) P Q :
+
+Theorem htriple_while_false (V : Set) (e1 e2 : Expr V) P Q :
   hoare_triple e1
     P
     (fun v c => <[v = Bool false]> <*> Q (1+(c+1))) ->
@@ -440,3 +580,21 @@ Theorem triple_while_false (V : Set) (e1 e2 : Expr V) P Q :
 Proof.
   solve_triple_15 big_red_while_false.
 Qed.
+(*
+Theorem htriple_while (V : Set) (e1 e2 : Expr V) n P Q :
+  (forall n,
+    hoare_triple e1
+      (P n)
+      (fun v c => <exists> b, <[v = Bool b]> <*> Q b n c)) ->
+  (forall n c,
+    hoare_triple e2
+      (Q true (S n) c)
+      (fun v c' => <[v = U_val]> <*> P n)) ->
+  hoare_triple (While e1 e2)
+    (P n)
+    (fun v c => <[v = U_val]> <*> Q false 0 c).
+Proof.
+  unfold_all. destruct n; simpl.
+  solve_triple_15 big_red_while_false.
+Qed.
+*)
